Minor refactoring

Ch3.v
@@ -6,47 +6,105 @@ From Coq Require Import ssreflect.
 Module Bool.
 
   Inductive term : Type :=
-  | true
-  | false
-  | ifelse : term -> term -> term -> term.
+  | T_true
+  | T_false
+  | T_cond (cond t1 t2 : term).
 
-  (* lets introduce a notation for expressiveness *)
-  Notation "'if' c 'then' t1 'else' t2" := (ifelse c t1 t2).
+  (* Let's introduce a custom grammar entry for expressiveness *)
 
-  (* evaluation relation on terms *)
+  Declare Custom Entry term.
+
+  Notation "[ e ]" := e (e custom term at level 2).
+  Notation "( x )" := x (in custom term, x at level 2).
+
+  Notation "'true'"  := (T_true)  (in custom term at level 0).
+  Notation "'false'" := (T_false) (in custom term at level 0).
+
+  Notation "'if' cond 'then' t1 'else' t2" :=
+    (T_cond cond t1 t2) (in custom term at level 2).
+
+  Notation "x" := x (in custom term at level 0, x constr at level 0).
+
+  Check [ true ].
+  Check fun cond t1 t2 => [ if cond then t1 else t2 ].
+  Unset Printing Notations.
+  Check fun cond t1 t2 => [ if cond then t1 else t2 ].
+  Set Printing Notations.
+
+  (* Evaluation relation on terms *)
   Reserved Notation "t ==> t'" (at level 50).
 
   Inductive eval_step : term -> term -> Prop :=
-  | E_IfTrue : forall t2 t3, (if true then t2 else t3) ==> t2
-  | E_IfFalse : forall t2 t3, (if false then t2 else t3) ==> t3
-  | E_If : forall t1 t1' t2 t3,
-      t1 ==> t1' -> (if t1 then t2 else t3) ==> (if t1' then t2 else t3)
-  where "t ==> t'" := (eval_step t t').
+  | E_IfTrue  : forall t1 t2, [ if true  then t1 else t2 ] ==> t1
+  | E_IfFalse : forall t1 t2, [ if false then t1 else t2 ] ==> t2
+  | E_If : forall c c' t1 t2, c ==> c' -> [ if c then t1 else t2] ==> [ if c' then t1 else t2 ]
+  where "e ==> e'" := (eval_step e e').
 
-  Example ex_inst_e_iftrue :
-    (if true then true else (if false then false else false)) ==> true.
+
+  Theorem ex_inst_e_iftrue :
+    [ if true then true else (if false then false else false) ] ==> [ true ].
   Proof.
-    apply E_IfTrue.
+    by apply: E_IfTrue.
   Qed.
 
-  Definition s := if true then false else false.
-  Definition t := if s then true else true.
-  Definition u := if false then true else true.
+  Module Ex_3_5_3.
+    Definition s := [ if true  then false else false ].
+    Definition t := [ if s     then true  else true  ].
+    Definition u := [ if false then true  else true  ].
 
-  Example ex3_5_3 :
-    (if t then false else false) ==> (if u then false else false).
-  Proof.
-    apply E_If.
-    apply E_If.
-    apply E_IfTrue.
-  Qed.
+    Theorem ex :
+      [ if t then false else false ] ==> [ if u then false else false ].
+    Proof.
+      apply: E_If.
+                     (*              t ==> u
+         [ if s then true else true  ] ==> [ if false then true else true  ] *)
+      apply: E_If.
+      (*                                 s ==> [ false ]
+         [ if true then false else false ] ==> [ false ] *)
+      exact: E_IfTrue.
 
-  Theorem one_step_eval_is_det :
+      (* Let's refactor it a bit *)
+      Restart.
+
+      by do 2! apply: E_If; exact: E_IfTrue.
+    Qed.
+  End Ex_3_5_3.
+
+  Theorem eval_step_is_det :
     forall t t' t'' : term,
       (t ==> t') /\ (t ==> t'') -> t' = t''.
-    Proof.
-      move => t t' t'' H.
-    Abort.
+  Proof.
+  (* I haven’t came up with a proof yet *)
+  Abort.
+
+  (* It would be much easier to define the
+     one-step evaluation as a function instead: *)
+
+  Fixpoint one_step (t : term) : term :=
+    match t with
+    | T_cond T_true t1 t2 => t1
+    | T_cond T_false t1 t2 => t2
+    | T_cond cond t1 t2 => T_cond (one_step cond) t1 t2
+    | t => t
+    end.
+
+  (* A separate notation, now for the
+     fixpoint-definition of one-step evaluation: *)
+
+  Notation "t ==>> t'" := (one_step t = t') (at level 50).
+
+  Theorem one_step_is_det t t' t'':
+    t ==>> t' /\ t ==>> t'' -> t' = t''.
+  Proof.
+    move=> [] H1 H2.
+    rewrite -H1 -H2.
+    done.
+
+    Restart.
+
+    (* Idiomatic proof *)
+    by move=> [] ->.
+  Qed.
 
 End Bool.
 
@@ -55,10 +113,10 @@ Module Arith.
   Inductive term : Type :=
   | term_true
   | term_false
-  | term_cond : term -> term -> term -> term
+  | term_cond (cond t1 t2 : term)
   | term_zero
-  | term_succ : term -> term
-  | term_pred : term -> term
-  | term_iszero : term -> term.
+  | term_succ (n : term)
+  | term_pred (n : term)
+  | term_iszero (n : term).
 
 End Arith.
